temp commit to merge in Arvind's comments

intermediate/Veritas.Intermediate.VerifyS.fst
@@ -10,11 +10,28 @@ let lemma_vget_simulates_SC
           (ensures (vtls_rel (vget s k v vs) (SC.vget s k v vs')))
   = ()
 
+let lemma_update_value_preserves_key_with_MAdd
+  (st:vstore)
+  (s:slot_id{store_contains st s}) 
+  (v:value_type_of (stored_key st s))
+  (k:key)
+  : Lemma (ensures store_contains_key_with_MAdd st k = store_contains_key_with_MAdd (update_value st s v) k)
+          [SMTPat (store_contains_key_with_MAdd (update_value st s v) k)]
+  = admit()
+
 let lemma_update_value_DVal_preserves_merkle_inv (st:vstore) (s:slot_id{store_contains st s /\ is_data_key (stored_key st s)}) (v:data_value)
   : Lemma (requires merkle_store_inv st)
           (ensures merkle_store_inv (update_value st s (DVal v)))
           [SMTPat (merkle_store_inv (update_value st s (DVal v)))]
-  = admit()
+  = let st' = update_value st s (DVal v) in
+    let aux1 (s':slot_id{store_contains st' s' /\ MVal? (stored_value st' s')})
+      : Lemma (in_store_flag_unset_equals_desc_not_in_store st' s')
+      = assert (in_store_flag_unset_equals_desc_not_in_store st s') in
+    let aux2 (s':slot_id{store_contains st' s' /\ MVal? (stored_value st' s')})
+      : Lemma (points_to_nearest_desc_in_store st' s')
+      = assert (points_to_nearest_desc_in_store st s') in
+    Classical.forall_intro aux1;
+    Classical.forall_intro aux2
 
 let lemma_vput_simulates_SC
       (vs:vtls{Valid? vs}) 
@@ -26,6 +43,91 @@ let lemma_vput_simulates_SC
           (ensures (vtls_rel (vput s k v vs) (SC.vput s k v vs'))) 
   = ()
 
+
+
+
+
+let lemma_add_to_store_preserves_key_with_MAdd (st:vstore) (s:st_index st{not (store_contains st s)}) (k:key) (v:value_type_of k) (k0:key)
+  : Lemma (requires k <> k0)
+          (ensures store_contains_key_with_MAdd st k0 = store_contains_key_with_MAdd (add_to_store st s k v Spec.MAdd) k0)
+          [SMTPat (store_contains_key_with_MAdd (add_to_store st s k v Spec.MAdd) k0)]
+  = admit()
+
+let lemma_add_to_store_adds_key_with_MAdd (st:vstore) (s:st_index st{not (store_contains st s)}) (k:key) (v:value_type_of k)
+  : Lemma (ensures store_contains_key_with_MAdd (add_to_store st s k v Spec.MAdd) k)
+          [SMTPat (store_contains_key_with_MAdd (add_to_store st s k v Spec.MAdd) k)]
+  = admit()
+
+let lemma_update_in_store_preserves_key_with_MAdd (st:vstore) (s:slot_id{store_contains st s}) (d:bin_tree_dir) (b:bool) (k:key)
+  : Lemma (ensures store_contains_key_with_MAdd st k = store_contains_key_with_MAdd (update_in_store st s d b) k)
+          [SMTPat (store_contains_key_with_MAdd (update_in_store st s d b) k)]
+  = admit()
+
+
+
+
+let lemma_addm_case1 (st:vstore) (s:st_index st) (s':slot_id{store_contains st s'}) (k:key)
+  : Lemma (requires (let k' = stored_key st s' in
+                     let v' = stored_value st s' in
+                     not (store_contains st s) /\
+                     MVal? v' /\ 
+                     is_proper_desc k k' /\
+                     Empty? (desc_hash_dir (to_merkle_value v') (desc_dir k k')) /\
+                     merkle_store_inv st))
+          (ensures (let v' = to_merkle_value (stored_value st s') in
+                    let d = desc_dir k (stored_key st s') in
+                    let h = hashfn (init_value k) in
+                    let v'_upd = Spec.update_merkle_value v' d k h false in
+                    let st_upd = update_value st s' (MVal v'_upd) in
+                    let st_upd2 = add_to_store st_upd s k (init_value k) Spec.MAdd in
+                    let st_upd3 = update_in_store st_upd2 s' d true in
+                    merkle_store_inv st_upd3))
+  = let k' = stored_key st s' in
+    let v' = to_merkle_value (stored_value st s') in
+    let d = desc_dir k (stored_key st s') in
+    let h = hashfn (init_value k) in
+    let v'_upd = Spec.update_merkle_value v' d k h false in
+    let st_upd = update_value st s' (MVal v'_upd) in
+    let st_upd2 = add_to_store st_upd s k (init_value k) Spec.MAdd in
+    let st_upd3 = update_in_store st_upd2 s' d true in
+    let aux1 (s0:slot_id{store_contains st_upd3 s0 /\ MVal? (stored_value st_upd3 s0)})
+      : Lemma (in_store_flag_unset_equals_desc_not_in_store st_upd3 s0)
+      = if s0 <> s
+        then (
+          assert (in_store_flag_unset_equals_desc_not_in_store st s0);
+          if s0 <> s'
+          then (
+            assert (points_to_nearest_desc_in_store st s0);
+            // points_to_nearest_desc_in_store implies the assumptions below, right?
+            let v0 = to_merkle_value (stored_value st s0) in
+            let dhl = desc_hash_dir v0 Left in
+            if Desc? dhl then assume (Desc?.k dhl <> k);
+            let dhr = desc_hash_dir v0 Right in
+            if Desc? dhr then assume (Desc?.k dhr <> k)
+          )
+        ) in
+    let aux2 (s0:slot_id{store_contains st_upd3 s0 /\ MVal? (stored_value st_upd3 s0)})
+      : Lemma (points_to_nearest_desc_in_store st_upd3 s0)
+      = if s0 = s 
+        then (
+          assert (points_to_nearest_desc_in_store st s');
+          let aux2_inner (k0:key{is_proper_desc k0 k})
+            : Lemma (not (store_contains_key_with_MAdd st_upd3 k0))
+            = lemma_proper_desc_transitive1 k0 k k';
+              lemma_two_related_desc_same_dir k0 k k' in
+          Classical.forall_intro aux2_inner
+        )
+        else (
+          assert (points_to_nearest_desc_in_store st s0);
+          if s0 = s'
+          then admit()
+          else admit()
+        ) in 
+    Classical.forall_intro aux1;
+    Classical.forall_intro aux2
+
+
+// The hard part here is showing that each case preserves merkle_store_inv
 #push-options "--z3rlimit_factor 2"
 let lemma_vaddm_simulates_SC 
       (vs:vtls{Valid? vs}) 
@@ -51,21 +153,13 @@ let lemma_vaddm_simulates_SC
           let st' = SC.thread_store vs' in
           match dh' with
           | Empty -> 
-              // CASE 1 - by points_to_nearest_desc_in_store, either k is not in the store or 
-              //          the final hash check is guaranteed to fail
+              // CASE 1 - k' has no descendent hash in direction d
               assert (points_to_nearest_desc_in_store st s');
-              if v = init_value k 
-              then (
-                let v'_upd = Spec.update_merkle_value v' d k h false in
-                let st_upd = update_value st s' (MVal v'_upd) in
-                let st_upd2 = add_to_store st_upd s k v Spec.MAdd in
-                let st_upd3 = update_in_store st_upd2 s' d true in
-                assume (merkle_store_inv st_upd3)
-              )
+              assert (not (store_contains_key_with_MAdd st k));
+              lemma_addm_case1 st s s' k
           | Desc k2 h2 b2 -> 
               if k2 = k 
-              // CASE 2 - by in_store_flag_implies.. and evicted_to_blum_flag_implies.., either 
-              //          k is not in the store or the final hash check is guaranteed to fail
+              // CASE 2 - k' has a descendent hash for k, and its in_store flag is not set           
               then (
                 assert (in_store_flag_unset_equals_desc_not_in_store st s');              
                 if h2 = h && b2 = false
@@ -78,11 +172,12 @@ let lemma_vaddm_simulates_SC
                   assume (merkle_store_inv st_upd2)
                 )
               )
-              // CASE 3 - similar to CASE 1
+              // CASE 3 - k' has a descendent hash for k2, and k is between k' and k2
               else (
                 assert (points_to_nearest_desc_in_store st s');              
                 if v = init_value k && is_proper_desc k2 k 
-                then
+                then (
+                  assert (not (store_contains_key_with_MAdd st k));
                   let d2 = desc_dir k2 k in
                   let mv = to_merkle_value v in
                   let mv_upd = Spec.update_merkle_value mv d2 k2 h2 b2 in
@@ -92,14 +187,63 @@ let lemma_vaddm_simulates_SC
                   let st_upd3 = update_in_store st_upd2 s' d true in
                   let st_upd4 = update_in_store st_upd3 s d2 true in
                   assume (merkle_store_inv st_upd4)
+                )
               )
 #pop-options
 
-let lemma_evict_from_store_preserves_inv (st:vstore) (s:slot_id{store_contains st s})
-  : Lemma (requires merkle_store_inv st)
-          (ensures merkle_store_inv (evict_from_store st s))
-          [SMTPat (merkle_store_inv (evict_from_store st s))]
+
+
+let lemma_evict_from_store_preserves_key_with_MAdd (st:vstore) (s:slot_id{store_contains st s}) (k:key)
+  : Lemma (requires stored_key st s <> k)
+          (ensures store_contains_key_with_MAdd st k = store_contains_key_with_MAdd (evict_from_store st s) k)
+          [SMTPat (store_contains_key_with_MAdd (evict_from_store st s) k)]
   = admit()
+
+let lemma_evictm_case1
+  (st:vstore)
+  (s:slot_id{store_contains st s}) 
+  (s':slot_id{store_contains st s'})
+  : Lemma (requires merkle_store_inv st /\ is_proper_desc (stored_key st s) (stored_key st s'))
+          (ensures (let d = desc_dir (stored_key st s) (stored_key st s') in
+                    let st_upd = evict_from_store st s in
+                    let st_upd2 = update_in_store st_upd s' d false in
+                    merkle_store_inv st_upd2))
+  = let d = desc_dir (stored_key st s) (stored_key st s') in
+    let st_upd = evict_from_store st s in
+    let st_upd2 = update_in_store st_upd s' d false in
+    let aux1 (s0:slot_id{store_contains st_upd2 s0 /\ MVal? (stored_value st_upd2 s0)})
+      : Lemma (in_store_flag_unset_equals_desc_not_in_store st_upd2 s0)
+      = assert (in_store_flag_unset_equals_desc_not_in_store st s0);
+        let v0 = to_merkle_value (stored_value st s0) in
+        let dhl = desc_hash_dir v0 Left in
+        let dhr = desc_hash_dir v0 Right in
+        if s0 <> s' 
+        then (
+          assert (stored_value st s0 = stored_value st_upd s0);
+          assert (stored_value st_upd s0 = stored_value st_upd2 s0);
+          assert (stored_key st s0 = stored_key st_upd2 s0);
+          if Desc? dhl
+          then (
+            assert (child_in_store st s0 Left = child_in_store st_upd2 s0 Left);
+            assume (Desc?.k dhl <> stored_key st s);
+            assert (store_contains_key_with_MAdd st (Desc?.k dhl) = store_contains_key_with_MAdd st_upd (Desc?.k dhl))
+          )
+        );
+        //else (
+        //  if Desc? dhl
+        //  then assert (child_in_store
+        //  admit()
+        //) 
+        admit() in
+    let aux2 (s0:slot_id{store_contains st_upd2 s0 /\ MVal? (stored_value st_upd2 s0)})
+      : Lemma (points_to_nearest_desc_in_store st_upd2 s0)
+      = admit() in //assert (points_to_nearest_desc_in_store st s') in
+    Classical.forall_intro aux1;
+    Classical.forall_intro aux2
+
+
+
+
 
 let lemma_has_in_store_merkle_desc (st:vstore) (st':SCstore.vstore) (s:slot_id{store_contains st s})
   : Lemma (requires equal_contents st st' /\ merkle_store_inv st)
@@ -116,7 +260,18 @@ let lemma_update_hash_and_blum_bit_preserves_inv
   : Lemma (requires merkle_store_inv st)
           (ensures merkle_store_inv (update_hash_and_blum_bit st s d h b)) 
           [SMTPat (merkle_store_inv (update_hash_and_blum_bit st s d h b))]
-  = admit()
+  = let mv = to_merkle_value (stored_value st s) in
+    let Desc k _ _ = desc_hash_dir mv d in
+    let mv' = Spec.update_merkle_value mv d k h b in
+    let st' = update_value st s (MVal mv') in
+    let aux1 (s':slot_id{store_contains st' s' /\ MVal? (stored_value st' s')})
+      : Lemma (in_store_flag_unset_equals_desc_not_in_store st' s')
+      = assert (in_store_flag_unset_equals_desc_not_in_store st s') in
+    let aux2 (s':slot_id{store_contains st' s' /\ MVal? (stored_value st' s')})
+      : Lemma (points_to_nearest_desc_in_store st' s')
+      = assert (points_to_nearest_desc_in_store st s') in
+    Classical.forall_intro aux1;
+    Classical.forall_intro aux2
 
 let lemma_vevictm_simulates_SC 
       (vs:vtls{Valid? vs}) 
@@ -124,7 +279,37 @@ let lemma_vevictm_simulates_SC
       (s s':slot_id)  
   : Lemma (requires (vtls_rel vs vs'))
           (ensures (vtls_rel (vevictm s s' vs) (SC.vevictm s s' vs'))) 
-  = ()
+  = let st = thread_store vs in
+    if store_contains st s && store_contains st s'
+    then 
+      let k = stored_key st s in
+      let v = stored_value st s in
+      let k' = stored_key st s' in
+      let v' = stored_value st s' in
+      if is_proper_desc k k' && not (has_instore_merkle_desc st s)
+      then
+        let d = desc_dir k k' in
+        let _ = assert (is_value_of k' v') in 
+        let v' = to_merkle_value v' in
+        let dh' = desc_hash_dir v' d in
+        let h = hashfn v in
+        match dh' with
+        | Empty -> ()
+        | Desc k2 h2 b2 -> 
+          if k2 = k 
+          then
+            let st_upd = update_hash_and_blum_bit st s' d h false in
+            let st_upd2 = evict_from_store st_upd s in
+            let st_upd3 = update_in_store st_upd2 s' d false in
+            assert (merkle_store_inv st_upd);
+            lemma_evictm st_upd s s'
+
+
+let lemma_add_to_store_BAdd_preserves_key_with_MAdd (st:vstore) (s:st_index st{not (store_contains st s)}) (k:key) (v:value_type_of k) (k0:key)
+  : Lemma (ensures store_contains_key_with_MAdd st k0 = store_contains_key_with_MAdd (add_to_store st s k v Spec.BAdd) k0)
+          [SMTPat (store_contains_key_with_MAdd (add_to_store st s k v Spec.BAdd) k0)]
+  = admit()
+
 
 let lemma_add_to_store_BAdd_preserves_inv (st:vstore) (s:st_index st{not (store_contains st s)}) (k:key) (v:value_type_of k)
   : Lemma (requires merkle_store_inv st)
@@ -142,6 +327,13 @@ let lemma_vaddb_simulates_SC
   : Lemma (requires (vtls_rel vs vs'))
           (ensures (vtls_rel (vaddb s r t j vs) (SC.vaddb s r t j vs')))
   = ()
+
+
+let lemma_evict_from_store_preserves_inv (st:vstore) (s:slot_id{store_contains st s})
+  : Lemma (requires merkle_store_inv st /\ add_method_of st s = Spec.BAdd)
+          (ensures merkle_store_inv (evict_from_store st s))
+          [SMTPat (merkle_store_inv (evict_from_store st s))]
+  = admit()
 
 let lemma_vevictb_simulates_SC 
       (vs:vtls{Valid? vs}) 
